Properties about successful searches (WIP)

correctness/RegexCorrectness/Backtracker/Traversal.lean
@@ -1,18 +1,24 @@
+import Regex.Strategy
 import RegexCorrectness.Backtracker.Basic
+import RegexCorrectness.Backtracker.Path
 
 set_option autoImplicit false
 
+open Regex.Data (Span BoundedIterator)
+
 namespace Regex.Backtracker.captureNextAux
 
-variable {σ nfa wf it startIdx maxIdx visited stack update visited'}
+section
+
+variable {σ nfa wf it startIdx maxIdx visited stack}
 
 theorem mem_of_mem_visited {s i} (hmem : visited.get s i) :
   (captureNextAux σ nfa wf startIdx maxIdx visited stack).2.get s i := by
   induction visited, stack using captureNextAux.induct' σ nfa wf startIdx maxIdx with
-  | base visited => simp [hmem]
-  | visited visited update state it eq stack' mem ih => simp [mem, ih hmem]
-  | done visited update state bit eq stack' mem hn => simp [mem, hn, BitMatrix.get_set, hmem]
-  | fail visited update state bit eq stack' mem hn => simp [mem, hn, BitMatrix.get_set, hmem]
+  | base visited => simp [captureNextAux_base, hmem]
+  | visited visited update state it eq stack' mem ih => simp [captureNextAux_visited mem, ih hmem]
+  | done visited update state it eq stack' mem hn => simp [captureNextAux_done mem hn, BitMatrix.get_set, hmem]
+  | fail visited update state it eq stack' mem hn => simp [captureNextAux_fail mem hn, BitMatrix.get_set, hmem]
   | epsilon visited update state it eq stack' mem visited' state' hn ih =>
     rw [captureNextAux_epsilon mem hn]
     exact ih (by simp [visited', BitMatrix.get_set, hmem])
@@ -52,15 +58,15 @@ theorem mem_of_mem_top_stack {entry stack'} (hstack : entry :: stack' = stack) :
   induction visited, stack using captureNextAux.induct' σ nfa wf startIdx maxIdx with
   | base visited => simp at hstack
   | visited visited update state it eq stack' mem ih =>
-    simp [mem]
+    simp [captureNextAux_visited mem]
     simp at hstack
     exact mem_of_mem_visited (by simp [hstack, mem])
-  | done visited update state bit eq stack' mem hn =>
-    simp [mem, hn]
+  | done visited update state it eq stack' mem hn =>
+    simp [captureNextAux_done mem hn]
     simp at hstack
     simp [hstack, BitMatrix.get_set]
-  | fail visited update state bit eq stack' mem hn =>
-    simp [mem, hn]
+  | fail visited update state it eq stack' mem hn =>
+    simp [captureNextAux_fail mem hn]
     simp at hstack
     simp [hstack, BitMatrix.get_set]
   | epsilon visited update state it eq stack'' mem visited' state' hn ih =>
@@ -107,5 +113,175 @@ theorem mem_of_mem_top_stack {entry stack'} (hstack : entry :: stack' = stack) :
     rw [captureNextAux_sparse_end mem hn hnext]
     simp at hstack
     exact mem_of_mem_visited (by simp [BitMatrix.get_set, hstack, mem])
+
+end
+
+section
+
+variable {nfa wf startIdx maxIdx visited stack update' visited'}
+
+/-
+TODO: add property of the visited so that we can know that visited is bounded by reachable states from the start node starting from a particular position.
+TODO: should we expand Path to take the starting span?
+-/
+structure UpperInv (wf : nfa.WellFormed) (stack : List (StackEntry HistoryStrategy nfa startIdx maxIdx)) where
+  reachable : ∀ entry ∈ stack, ∃ span, span.iterator = entry.it.it ∧ Path nfa wf span entry.state entry.update
+
+theorem path_done_of_some (hres : captureNextAux HistoryStrategy nfa wf startIdx maxIdx visited stack = (.some update', visited'))
+  (inv : UpperInv wf stack) :
+  ∃ state span, nfa[state] = .done ∧ Path nfa wf span state update' := by
+  induction visited, stack using captureNextAux.induct' HistoryStrategy nfa wf startIdx maxIdx with
+  | base visited => simp [captureNextAux_base] at hres
+  | visited visited update state it eq stack' mem ih =>
+    simp [captureNextAux_visited mem] at hres
+    have inv' : UpperInv wf stack' := by
+      have reachable entry (mem : entry ∈ stack') : ∃ span, span.iterator = entry.it.it ∧ Path nfa wf span entry.state entry.update :=
+        inv.reachable entry (by simp [mem])
+      exact ⟨reachable⟩
+    exact ih hres inv'
+  | done visited update state it eq stack' mem hn =>
+    simp [captureNextAux_done mem hn] at hres
+    have ⟨span, eqspan, path⟩ := inv.reachable ⟨update, state, it, eq⟩ (by simp)
+    exact ⟨state, span, hn, hres.1 ▸ path⟩
+  | fail visited update state it eq stack' mem hn => simp [captureNextAux_fail mem hn] at hres
+  | epsilon visited update state it eq stack' mem visited' state' hn ih =>
+    rw [captureNextAux_epsilon mem hn] at hres
+    have inv' : UpperInv wf (⟨update, state', it, eq⟩ :: stack') := by
+      have reachable entry (mem : entry ∈ ⟨update, state', it, eq⟩ :: stack') : ∃ span, span.iterator = entry.it.it ∧ Path nfa wf span entry.state entry.update := by
+        simp at mem
+        cases mem with
+        | inl eq' =>
+          subst entry
+          have ⟨span, eqspan, path⟩ := inv.reachable ⟨update, state, it, eq⟩ (by simp)
+          simp at eqspan path
+          exact ⟨span, by simp [eqspan], path.more (.epsilon (Nat.zero_le _) state.isLt hn) (by simp)⟩
+        | inr mem => exact inv.reachable entry (by simp [mem])
+      exact ⟨reachable⟩
+    exact ih hres inv'
+  | split visited update state it eq stack' mem visited' state₁ state₂ hn ih =>
+    rw [captureNextAux_split mem hn] at hres
+    let stack'' := ⟨update, state₁, it, eq⟩ :: ⟨update, state₂, it, eq⟩ :: stack'
+    have inv' : UpperInv wf stack'' := by
+      have reachable entry (mem : entry ∈ stack'') : ∃ span, span.iterator = entry.it.it ∧ Path nfa wf span entry.state entry.update := by
+        simp [stack''] at mem
+        match mem with
+        | .inl eq₁ =>
+          subst entry
+          have ⟨span, eqspan, path⟩ := inv.reachable ⟨update, state, it, eq⟩ (by simp)
+          simp at eqspan path
+          exact ⟨span, by simp [eqspan], path.more (.splitLeft (Nat.zero_le _) state.isLt hn) (by simp)⟩
+        | .inr (.inl eq₂) =>
+          subst entry
+          have ⟨span, eqspan, path⟩ := inv.reachable ⟨update, state, it, eq⟩ (by simp)
+          simp at eqspan path
+          exact ⟨span, by simp [eqspan], path.more (.splitRight (Nat.zero_le _) state.isLt hn) (by simp)⟩
+        | .inr (.inr mem) => exact inv.reachable entry (by simp [mem])
+      exact ⟨reachable⟩
+    exact ih hres inv'
+  | save visited update state it eq stack' mem visited' offset state' hn update' ih =>
+    rw [captureNextAux_save mem hn] at hres
+    have inv' : UpperInv wf (⟨update', state', it, eq⟩ :: stack') := by
+      have reachable entry (mem : entry ∈ ⟨update', state', it, eq⟩ :: stack') : ∃ span, span.iterator = entry.it.it ∧ Path nfa wf span entry.state entry.update := by
+        simp at mem
+        cases mem with
+        | inl eq' =>
+          subst entry
+          have ⟨span, eqspan, path⟩ := inv.reachable ⟨update, state, it, eq⟩ (by simp)
+          simp at eqspan path
+          exact ⟨span, by simp [eqspan], path.more (.save (Nat.zero_le _) state.isLt hn) (by simp [update', HistoryStrategy, BoundedIterator.pos, ←eqspan, Span.curr_eq_pos])⟩
+        | inr mem => exact inv.reachable entry (by simp [mem])
+      exact ⟨reachable⟩
+    exact ih hres inv'
+  | anchor_pos visited update state it eq stack' mem visited' a state' hn ht ih =>
+    rw [captureNextAux_anchor_pos mem hn ht] at hres
+    have inv' : UpperInv wf (⟨update, state', it, eq⟩ :: stack') := by
+      have reachable entry (mem : entry ∈ ⟨update, state', it, eq⟩ :: stack') : ∃ span, span.iterator = entry.it.it ∧ Path nfa wf span entry.state entry.update := by
+        simp at mem
+        cases mem with
+        | inl eq' =>
+          subst entry
+          have ⟨span, eqspan, path⟩ := inv.reachable ⟨update, state, it, eq⟩ (by simp)
+          simp at eqspan path
+          exact ⟨span, by simp [eqspan], path.more (.anchor (Nat.zero_le _) state.isLt hn (eqspan ▸ ht)) (by simp)⟩
+        | inr mem => exact inv.reachable entry (by simp [mem])
+      exact ⟨reachable⟩
+    exact ih hres inv'
+  | anchor_neg visited update state it eq stack' mem visited' a state' hn ht ih =>
+    rw [captureNextAux_anchor_neg mem hn ht] at hres
+    have inv' : UpperInv wf stack' := by
+      have reachable entry (mem : entry ∈ stack') : ∃ span, span.iterator = entry.it.it ∧ Path nfa wf span entry.state entry.update :=
+        inv.reachable entry (by simp [mem])
+      exact ⟨reachable⟩
+    exact ih hres inv'
+  | char_pos visited update state it eq stack' mem visited' c state' hn hnext hc ih =>
+    rw [captureNextAux_char_pos mem hn hnext hc] at hres
+    have inv' : UpperInv wf (⟨update, state', it.next hnext, eq⟩ :: stack') := by
+      have reachable entry (mem : entry ∈ ⟨update, state', it.next hnext, eq⟩ :: stack') : ∃ span, span.iterator = entry.it.it ∧ Path nfa wf span entry.state entry.update := by
+        simp at mem
+        cases mem with
+        | inl eq' =>
+          subst entry
+          have ⟨span, eqspan, path⟩ := inv.reachable ⟨update, state, it, eq⟩ (by simp)
+          simp at eqspan path
+          simp [BoundedIterator.hasNext, BoundedIterator.curr, ←eqspan] at hnext hc
+          have ⟨r', eqr'⟩ := span.exists_cons_of_curr' hnext hc
+          refine ⟨span.next, by simp [span.next_iterator eqr', eqspan, BoundedIterator.next, String.Iterator.next'_eq_next], ?_⟩
+          simp
+          have step : NFA.Step nfa 0 state span state' span.next .none := by
+            simp [NFA.Step.iff_char hn, eqr', span.next_eq eqr']
+          exact path.more step (by simp)
+        | inr mem => exact inv.reachable entry (by simp [mem])
+      exact ⟨reachable⟩
+    exact ih hres inv'
+  | char_neg visited update state it eq stack' mem visited' c state' hn hnext hc ih =>
+    rw [captureNextAux_char_neg mem hn hnext hc] at hres
+    have inv' : UpperInv wf stack' := by
+      have reachable entry (mem : entry ∈ stack') : ∃ span, span.iterator = entry.it.it ∧ Path nfa wf span entry.state entry.update :=
+        inv.reachable entry (by simp [mem])
+      exact ⟨reachable⟩
+    exact ih hres inv'
+  | char_end visited update state it eq stack' mem visited' c state' hn hnext ih =>
+    rw [captureNextAux_char_end mem hn hnext] at hres
+    have inv' : UpperInv wf stack' := by
+      have reachable entry (mem : entry ∈ stack') : ∃ span, span.iterator = entry.it.it ∧ Path nfa wf span entry.state entry.update :=
+        inv.reachable entry (by simp [mem])
+      exact ⟨reachable⟩
+    exact ih hres inv'
+  | sparse_pos visited update state it eq stack' mem visited' cs state' hn hnext hc ih =>
+    rw [captureNextAux_sparse_pos mem hn hnext hc] at hres
+    have inv' : UpperInv wf (⟨update, state', it.next hnext, eq⟩ :: stack') := by
+      have reachable entry (mem : entry ∈ ⟨update, state', it.next hnext, eq⟩ :: stack') : ∃ span, span.iterator = entry.it.it ∧ Path nfa wf span entry.state entry.update := by
+        simp at mem
+        cases mem with
+        | inl eq' =>
+          subst entry
+          have ⟨span, eqspan, path⟩ := inv.reachable ⟨update, state, it, eq⟩ (by simp)
+          simp at eqspan path
+          simp [BoundedIterator.hasNext, BoundedIterator.curr, ←eqspan] at hnext hc
+          have ⟨r', eqr'⟩ := span.exists_cons_of_curr' hnext rfl
+          refine ⟨span.next, by simp [span.next_iterator eqr', eqspan, BoundedIterator.next, String.Iterator.next'_eq_next], ?_⟩
+          simp
+          have step : NFA.Step nfa 0 state span state' span.next .none := by
+            simp [NFA.Step.iff_sparse hn, eqr', span.next_eq eqr', hc]
+          exact path.more step (by simp)
+        | inr mem => exact inv.reachable entry (by simp [mem])
+      exact ⟨reachable⟩
+    exact ih hres inv'
+  | sparse_neg visited update state it eq stack' mem visited' cs state' hn hnext hc ih =>
+    rw [captureNextAux_sparse_neg mem hn hnext hc] at hres
+    have inv' : UpperInv wf stack' := by
+      have reachable entry (mem : entry ∈ stack') : ∃ span, span.iterator = entry.it.it ∧ Path nfa wf span entry.state entry.update :=
+        inv.reachable entry (by simp [mem])
+      exact ⟨reachable⟩
+    exact ih hres inv'
+  | sparse_end visited update state it eq stack' mem visited' cs state' hn hnext ih =>
+    rw [captureNextAux_sparse_end mem hn hnext] at hres
+    have inv' : UpperInv wf stack' := by
+      have reachable entry (mem : entry ∈ stack') : ∃ span, span.iterator = entry.it.it ∧ Path nfa wf span entry.state entry.update :=
+        inv.reachable entry (by simp [mem])
+      exact ⟨reachable⟩
+    exact ih hres inv'
+
+end
 
 end Regex.Backtracker.captureNextAux
