correctness/RegexCorrectness/Backtracker/Compile.lean
@@ -1,0 +1,55 @@
+import RegexCorrectness.Data.BoundedIterator
+import RegexCorrectness.Data.Span
+import RegexCorrectness.Backtracker.Traversal
+import RegexCorrectness.NFA.Semantics
+
+set_option autoImplicit false
+
+open String (Pos)
+open Regex.NFA (EquivUpdate)
+open Regex.Data (BoundedIterator Span)
+
+namespace Regex.Backtracker
+
+theorem captureNext.go.path_done_of_some {nfa wf startIdx bit} {update} {visited visited' : BitMatrix nfa.nodes.size (bit.maxIdx + 1 - startIdx)}
+  (v : bit.Valid) (hres : captureNext.go HistoryStrategy nfa wf startIdx bit visited = (.some update, visited')) :
+  ∃ state span, nfa[state] = .done ∧ Path nfa wf span state update := by
+  induction bit, visited using captureNext.go.induct' HistoryStrategy nfa wf startIdx with
+  | found bit visited update' visited' haux =>
+    simp [captureNext.go_found haux] at hres
+    simp [hres] at haux
+    have inv₀ : captureNextAux.UpperInv wf [⟨[], ⟨nfa.start, wf.start_lt⟩, bit, rfl⟩] := by
+      refine ⟨?_⟩
+      simp
+      have ⟨l, r, vf⟩ := (bit.valid_of_valid v).validFor
+      exact ⟨⟨l.reverse, [], r⟩, (Span.validFor ⟨l.reverse, [], r⟩).eq_it (by simp [vf]), .init⟩
+    exact captureNextAux.path_done_of_some haux inv₀
+  | not_found_next bit visited visited' haux hnext ih =>
+    simp [captureNext.go_not_found_next haux hnext] at hres
+    exact ih (bit.next_valid hnext v) hres
+  | not_found_end bit visited visited' haux hnext => simp [captureNext.go_not_found_end haux hnext] at hres
+
+theorem captureNext.path_done_of_some {nfa wf it update} (hres : captureNext HistoryStrategy nfa wf it = .some update) (v : it.Valid) :
+  ∃ state span, nfa[state] = .done ∧ Path nfa wf span state update := by
+  if le : it.pos ≤ it.toString.endPos then
+    simp [captureNext_le le] at hres
+    let result := go HistoryStrategy nfa wf it.pos.byteIdx ⟨it, (Nat.le_refl _), le⟩ (BitMatrix.zero _ _)
+    change result.1 = .some update at hres
+    have : result = (.some update, result.2) := by simp [Prod.ext_iff, hres]
+    exact captureNext.go.path_done_of_some (BoundedIterator.valid_of_it_valid _ v) this
+  else
+    simp [captureNext_not_le le] at hres
+
+theorem captureNext.capture_of_some_compile {e it update} (hres : captureNext HistoryStrategy (NFA.compile e) NFA.compile_wf it = .some update) (v : it.Valid) :
+  ∃ l r span groups,
+    span.toString = it.toString ∧
+    e.Captures ⟨l, [], r⟩ span groups ∧
+    EquivUpdate groups update := by
+  have ⟨state, span, hn, path⟩ := captureNext.path_done_of_some hres v
+  have eq_zero := (NFA.done_iff_zero_compile rfl state).mp hn
+  have ne : state.val ≠ (NFA.compile e).start := eq_zero ▸ Nat.ne_of_lt (NFA.lt_zero_start_compile rfl)
+  have ⟨l, r, path⟩ := path.nfaPath_of_ne ne
+  have ⟨groups, eqv, c⟩ := NFA.captures_of_path_compile rfl (eq_zero ▸ path.compile_liftBound rfl)
+  exact ⟨l, r, span, groups, sorry, c, eqv⟩
+
+end Regex.Backtracker
