correctness/RegexCorrectness/Backtracker/Path.lean
@@ -1,0 +1,44 @@
+import RegexCorrectness.NFA.Semantics.Path
+
+set_option autoImplicit false
+
+open Regex.Data (Span)
+
+namespace Regex.Backtracker
+
+inductive Path (nfa : NFA) (wf : nfa.WellFormed) : Span → Fin nfa.nodes.size → List (Nat × String.Pos) → Prop where
+  | init {l r} : Path nfa wf ⟨l, [], r⟩ ⟨nfa.start, wf.start_lt⟩ []
+  | more {i j : Fin nfa.nodes.size} {span₁ span₂ update₁ update₂ update₃} (prev : Path nfa wf span₁ i update₁) (step : nfa.Step 0 i span₁ j span₂ update₂)
+    (equpdate : update₃ = update₁ ++ List.ofOption update₂) :
+    Path nfa wf span₂ j update₃
+
+namespace Path
+
+theorem eq_or_nfaPath {nfa : NFA} {wf : nfa.WellFormed} {span i update} (path : Path nfa wf span i update) :
+  ∃ l r,
+    (span = ⟨l, [], r⟩ ∧ i.val = nfa.start ∧ update = []) ∨
+    nfa.Path 0 nfa.start ⟨l, [], r⟩ i span update := by
+  induction path with
+  | @init l r =>
+    exists l, r
+    simp
+  | @more i j span₁ span₂ update₁ update₂ update₃ prev step equpdate ih =>
+    have ⟨l, r, h⟩ := ih
+    exists l, r
+    match h with
+    | .inl ⟨eqspan, eqi, equpdate'⟩ =>
+      simp [equpdate, equpdate']
+      exact .inr (.last (eqspan ▸ eqi ▸ step))
+    | .inr path =>
+      simp [equpdate]
+      exact .inr (path.trans (.last step))
+
+theorem nfaPath_of_ne {nfa : NFA} {wf : nfa.WellFormed} {span i update} (path : Path nfa wf span i update) (ne : i.val ≠ nfa.start) :
+  ∃ l r, nfa.Path 0 nfa.start ⟨l, [], r⟩ i span update := by
+  have ⟨l, r, h⟩ := eq_or_nfaPath path
+  simp [ne] at h
+  exact ⟨l, r, h⟩
+
+end Path
+
+end Regex.Backtracker
